theories/logrel/lib/list.v
@@ -1,0 +1,75 @@
+From actris.utils Require Import llist.
+From actris.channel Require Import proofmode.
+From actris.logrel Require Import term_types.
+
+Definition lty_list_aux `{!heapG Σ} (A : ltty Σ) (X : ltty Σ) : ltty Σ :=
+  ref_uniq (() + (A * X)).
+Instance lty_list_aux_contractive `{!heapG Σ} A :
+  Contractive (@lty_list_aux Σ _ A).
+Proof. solve_proto_contractive. Qed.
+Definition lty_list `{!heapG Σ} (A : ltty Σ) : ltty Σ := lty_rec (lty_list_aux A).
+
+Notation "'list' A" := (lty_list A) (at level 10) : lty_scope.
+
+Section with_Σ.
+  Context `{!heapG Σ}.
+
+  Lemma list_type_loc A v :
+    ltty_car (list A) v -∗ ∃ (l : loc) , ⌜v = #l⌝.
+  Proof.
+    iIntros "Hv". rewrite /lty_list /lty_rec fixpoint_unfold.
+    iDestruct "Hv" as (l v' Heq) "Hv". by iExists l.
+  Qed.
+
+  Definition llist_type_pred (A : ltty Σ) : val → val → iProp Σ :=
+    (λ v w : val, ⌜v = w⌝ ∗ ltty_car A v)%I.
+
+  Lemma llist_lty_list lys ys A :
+    llist (llist_type_pred A) lys ys -∗
+          ltty_car (lty_list A) #lys.
+  Proof.
+    iIntros "Hlys".
+    iInduction ys as [|y ys] "IH" forall (lys).
+    - rewrite /lty_list /lty_rec fixpoint_unfold.
+      iExists lys, NONEV. rewrite /llist. iFrame "Hlys".
+      iSplit; [ done | ].
+      iLeft. eauto.
+    - iDestruct "Hlys" as (vb l'') "[[-> HB] [Hl' Hrec]]".
+      iEval (rewrite /lty_list /lty_rec fixpoint_unfold).
+      iExists lys, _. iFrame "Hl'".
+      iSplit; [ done | ].
+      rewrite /lty_list /lty_rec.
+      iRight. iExists _. iSplit; [ done | ]. iExists _, _. iSplit; [ done | ].
+      iFrame "HB". by iApply ("IH" with "Hrec").
+  Qed.
+
+  Lemma llength_spec A (l : loc) :
+    ⊢ {{{ ltty_car (list A) #l }}} llength #l
+      {{{ xs (n:Z), RET #n; ⌜Z.of_nat (length xs) = n⌝ ∗
+                            llist (llist_type_pred A) l xs }}}.
+  Proof.
+    iIntros "!>" (Φ) "Hl HΦ".
+    iLöb as "IH" forall (l Φ).
+    wp_lam.
+    rewrite {2}/lty_list /lty_rec /lty_list_aux fixpoint_unfold.
+    iDestruct "Hl" as (ltmp l' [=<-]) "[Hl [ Hl' | Hl' ]]".
+    - wp_load. iDestruct "Hl'" as (xs ->) "Hl'". wp_pures.
+      iAssert (llist (llist_type_pred A) l [])%I with "[Hl Hl']" as "Hl".
+      { rewrite /llist. iDestruct "Hl'" as %->. iApply "Hl". }
+      iApply "HΦ". eauto with iFrame.
+    - wp_load. iDestruct "Hl'" as (xs ->) "Hl'". wp_pures.
+      iDestruct "Hl'" as (x vl' ->) "[HA Hl']".
+      wp_pures.
+      rewrite fixpoint_unfold.
+      iDestruct "Hl'" as (l' xs ->) "[Hl' Hl'']".
+      wp_apply ("IH" with "[Hl' Hl'']").
+      { rewrite /lty_list /lty_rec.
+        iEval (rewrite fixpoint_unfold).
+        iExists _, _. iFrame "Hl' Hl''". done. }
+      iIntros (ys n) "[<- H]".
+      iAssert (llist (llist_type_pred A) l (x :: ys))%I with "[Hl HA H]" as "Hl".
+      { iExists x, l'. eauto with iFrame. }
+      wp_pures. iApply "HΦ". iFrame "Hl". by rewrite (Nat2Z.inj_add 1).
+  Qed.
+
+End with_Σ.
